Eff orset

new/ORSet_rid_map.fst
@@ -2,6 +2,9 @@ module Orset_rid_map
 
 module M = Map_extended
 module S = FStar.Set
+open SeqUtils
+open FStar.Seq
+open FStar.Ghost
 module E = Ewflag_rid_map
 
 #set-options "--query_stats"
@@ -44,18 +47,86 @@ type timestamp_t = pos
 
 type op_t = timestamp_t & (nat (*replica_id*) & app_op_t)
 
+let get_rid (_,(rid,_)) = rid
+
+type log = seq op_t
+
+let mem_rid (rid:nat) (l:log) =
+  exists e. mem e l /\ fst (snd e) = rid
+
+unfold
+let ( ++ ) (l1 l2:log) = Seq.append l1 l2
+
+unfold
+let mem_id (id:timestamp_t) (l:log) : bool =
+  mem_assoc_fst id l
+  
+unfold
+let distinct_ops (l:log) = distinct_assoc_fst l
+
+type st0 = concrete_st & erased log
+  
+let v_of (s:st0) : concrete_st = fst s
+let ops_of (s:st0) : GTot log = snd s
+
 let get_ele (o:op_t) =
   match o with
   |(_,(_,Add ele)) -> ele
   |(_,(_,Rem ele)) -> ele
 
-let get_rid (_,(rid,_)) = rid
-
 // apply an operation to a state
-let do (s:concrete_st) (o:op_t) : concrete_st =
+let do (s:concrete_st) (o:op_t) 
+  : (r:concrete_st{(forall rid e. e <> get_ele o ==> E.sel (sel r e) rid = E.sel (sel s e) rid) /\
+                   (Add? (snd (snd o)) ==> (forall e. M.contains r e <==> M.contains s e \/ e = get_ele o) /\
+                                   (forall e. e = get_ele o ==> E.sel (sel r e) (get_rid o) = (fst (E.sel (sel s e) (get_rid o)) + 1, true))) /\
+                   (Rem? (snd (snd o)) ==> (forall e. M.contains r e <==> M.contains s e) /\
+                                   (forall e rid. e = get_ele o ==> E.sel (sel r e) rid = (fst (E.sel (sel s e) rid), false)))}) =
   match o with
   |(_, (rid, Add e)) -> M.upd s e (M.upd (sel s e) rid (fst (E.sel (sel s e) rid) + 1, true))
   |(_, (rid, Rem e)) -> M.iter_upd (fun k v -> if k = get_ele o then ((M.map_val (fun (c,f) -> (c, false))) v) else v) s
+
+#push-options "--ifuel 3"
+let lem_do (a b:concrete_st) (op:op_t)
+   : Lemma (requires eq a b)
+           (ensures eq (do a op) (do b op)) = ()
+#pop-options
+
+// applying a log of operations to a concrete state
+let rec apply_log (x:concrete_st) (l:log) : Tot concrete_st (decreases length l) =
+  match length l with
+  |0 -> x
+  |_ -> apply_log (do x (head l)) (tail l)                   
+
+// property of apply_log
+let rec lem_apply_log (x:concrete_st) (l:log)
+  : Lemma (ensures (length l > 0 ==> apply_log x l == do (apply_log x (fst (un_snoc l))) (last l)))
+          (decreases length l) =
+  match length l with
+  |0 -> ()
+  |_ -> lem_apply_log (do x (head l)) (tail l)
+
+#push-options "--z3rlimit 50 --ifuel 3"
+let rec lem_apply (x:concrete_st) (l:log)
+  : Lemma (ensures (let r = apply_log x l in
+                        //(forall rid. M.contains r rid ==> M.contains x rid \/ mem_rid rid l) /\
+                        (forall ele. M.contains x ele ==> M.contains r ele) /\
+                        (forall ele. M.contains x ele ==> (forall rid. M.contains (sel x ele) rid ==> M.contains (sel r ele) rid)) /\ 
+                        (forall ele rid. M.contains x ele /\ M.contains (sel x ele) rid ==> fst (E.sel (sel r ele) rid) >= fst (E.sel (sel x ele) rid))))
+                        //(forall rid. fst (sel r rid) >= fst (sel x rid))))
+          (decreases length l) =
+          //[SMTPat (apply_log x l)] =
+  match length l with
+  |0 -> ()
+  |_ -> lem_apply (do x (head l)) (tail l)
+#pop-options
+
+type st1 = s:st0{(v_of s == apply_log init_st (ops_of s))}
+
+let valid_st (s:st0) : prop =
+  distinct_ops (ops_of s) /\
+  (v_of s == apply_log init_st (ops_of s))
+
+type st = s:st0{valid_st s}
 
 type resolve_conflict_res =
   | First_then_second // op2.op1 
@@ -65,10 +136,1306 @@ let resolve_conflict (x:op_t) (y:op_t{fst x <> fst y}) : resolve_conflict_res =
   if get_ele x = get_ele y && Add? (snd (snd x)) && Rem? (snd (snd y)) then First_then_second 
   else Second_then_first
 
-let concrete_merge (lca s1 s2:concrete_st) : concrete_st =  
+let concrete_merge (lca s1 s2:concrete_st) 
+  : (r:concrete_st{(forall e. M.contains r e <==> M.contains lca e \/ M.contains s1 e \/ M.contains s2 e) /\
+                   (forall e rid. E.sel (sel r e) rid = E.sel (E.concrete_merge (sel lca e) (sel s1 e) (sel s2 e)) rid)}) =  
   let eles = S.union (M.domain lca) (S.union (M.domain s1) (M.domain s2)) in
   let u = M.const_on eles init_st in
   M.iter_upd (fun k v -> E.concrete_merge (sel lca k) (sel s1 k) (sel s2 k)) u
+
+//operations x and y are commutative
+let commutative (x y:op_t) =
+  not (((Add? (snd (snd x)) && Rem? (snd (snd y)) && get_ele x = get_ele y) ||
+        (Add? (snd (snd y)) && Rem? (snd (snd x)) && get_ele x = get_ele y))) 
+
+let comm_symmetric (x y:op_t) 
+  : Lemma (requires commutative x y)
+          (ensures commutative y x) = ()
+          
+// if x and y are commutative ops, applying them in any order should give equivalent results
+let commutative_prop (x y:op_t) 
+  : Lemma (requires commutative x y)
+          (ensures (forall s. eq (apply_log s (cons x (cons y empty))) (apply_log s (cons y (cons x empty))))) = ()
+
+//commutativity for a sequence of operation
+let commutative_seq (x:op_t) (l:log) : bool =
+  forallb (fun e -> commutative x e) l
+
+let comm_empty_log (x:op_t) (l:log)
+  : Lemma (ensures length l = 0 ==> commutative_seq x l) = ()
+  
+let inverse_st (s:st{Seq.length (ops_of s) > 0}) 
+  : GTot (i:st{(v_of s == do (v_of i) (last (ops_of s))) /\
+               (ops_of i = fst (un_snoc (ops_of s))) /\
+               (ops_of s = snoc (ops_of i) (last (ops_of s))) /\
+               is_prefix (ops_of i) (ops_of s) /\
+               (forall id. mem_id id (ops_of i) <==> mem_id id (ops_of s) /\ id <> fst (last (ops_of s)))}) =
+  let p,_ = un_snoc (ops_of s) in
+  let r = apply_log init_st p in
+  lem_apply_log init_st (ops_of s);
+  let p, l = un_snoc (ops_of s) in
+  let r = apply_log init_st p in
+  lemma_split (ops_of s) (length (ops_of s) - 1); 
+  lemma_append_count_assoc_fst p (snd (split (ops_of s) (length (ops_of s) - 1))); 
+  distinct_invert_append p (snd (split (ops_of s) (length (ops_of s) - 1)));
+  (r, hide p)
+
+//currently present in App.fsti as Log MRDT needs it
+let rec inverse_helper (s:concrete_st) (l':log) (op:op_t)
+  : Lemma (ensures (let l = Seq.snoc l' op in 
+                   (apply_log s l == do (apply_log s l') op))) 
+          (decreases length l')
+  = Seq.un_snoc_snoc l' op;
+    match length l' with
+    |0 -> ()
+    |_ -> inverse_helper (do s (head l')) (tail l') op
+  
+//currently present in App.fsti as Log MRDT needs it
+let rec split_prefix (s:concrete_st) (l:log) (a:log)
+  : Lemma (requires is_prefix l a)
+          (ensures (apply_log s a == apply_log (apply_log s l) (diff a l)) /\
+                   (forall e. mem e l ==> mem e a) /\
+                   (Seq.length a > Seq.length l ==> (last a) == (last (diff a l))))
+          (decreases Seq.length l)
+  = match Seq.length l with
+    |0 -> ()
+    |_ -> split_prefix (do s (head l)) (tail l) (tail a)
+
+let consistent_branches (lca s1 s2:st1) =
+  distinct_ops (ops_of lca) /\ distinct_ops (ops_of s1) /\ distinct_ops (ops_of s2) /\
+  is_prefix (ops_of lca) (ops_of s1) /\
+  is_prefix (ops_of lca) (ops_of s2) /\
+  (forall id id1. mem_id id (ops_of lca) ==> not (mem_id id1 (diff (ops_of s1) (ops_of lca)))) /\
+  (forall id id1. mem_id id (ops_of lca) ==> not (mem_id id1 (diff (ops_of s2) (ops_of lca)))) /\
+  (forall id. mem_id id (diff (ops_of s1) (ops_of lca)) ==> not (mem_id id (diff (ops_of s2) (ops_of lca)))) /\
+  (forall rid. mem_rid rid (diff (ops_of s1) (ops_of lca)) ==> ~ (mem_rid rid (diff (ops_of s2) (ops_of lca))))
+
+let consistent_branches_s1_gt0 (lca s1 s2:st1) =
+  consistent_branches lca s1 s2 /\
+  length (ops_of s1) > length (ops_of lca)
+
+let consistent_branches_s2_gt0 (lca s1 s2:st1) =
+  consistent_branches lca s1 s2 /\
+  length (ops_of s2) > length (ops_of lca)
+
+let consistent_branches_s1s2_gt0 (lca s1 s2:st1) =
+  consistent_branches lca s1 s2 /\
+  length (ops_of s1) > length (ops_of lca) /\
+  length (ops_of s2) > length (ops_of lca)
+
+let do_st (s:st1) (o:op_t) : st1 =
+  split_prefix init_st (ops_of s) (snoc (ops_of s) o); 
+  (do (v_of s) o, hide (snoc (ops_of s) o))
+
+let merge_is_comm (lca s1 s2:st)
+  : Lemma (requires true) //consistent_branches lca s1 s2)
+          (ensures (eq (concrete_merge (v_of lca) (v_of s1) (v_of s2)) 
+                       (concrete_merge (v_of lca) (v_of s2) (v_of s1)))) = ()
+
+let lem_trans_merge_s1' (lca s1 s2 s1':concrete_st)
+  : Lemma (requires eq s1 s1')
+          (ensures eq (concrete_merge lca s1 s2)
+                      (concrete_merge lca s1' s2)) = ()
+
+let lem_trans_merge_s2' (lca s1 s2 s2':concrete_st)
+  : Lemma (requires eq s2 s2')
+          (ensures eq (concrete_merge lca s1 s2)
+                      (concrete_merge lca s1 s2')) = ()
+                      
+let linearizable_s1_0 (lca s1 s2:st)
+  : Lemma (requires consistent_branches lca s1 s2 /\
+                    ops_of s1 == ops_of lca)
+          (ensures eq (v_of s2) (concrete_merge (v_of lca) (v_of s1) (v_of s2))) = admit()
+
+let pre1_pre2_s2 (lca s1 s2:st)
+    : Lemma (requires consistent_branches_s2_gt0 lca s1 s2)
+            (ensures consistent_branches lca s1 (inverse_st s2)) = 
+  lem_inverse (ops_of lca) (ops_of s2);
+  lastop_diff (ops_of lca) (ops_of s2);
+  inverse_diff_id_s2' (ops_of lca) (ops_of s1) (ops_of s2);
+  assume (forall rid. mem_rid rid (diff (ops_of s1) (ops_of lca)) ==> ~ (mem_rid rid (diff (fst (un_snoc (ops_of s2))) (ops_of lca)))); ()
+
+let pre1_pre2_s1 (lca s1 s2:st)
+    : Lemma (requires consistent_branches_s1_gt0 lca s1 s2)
+            (ensures consistent_branches lca (inverse_st s1) s2) = 
+  lem_inverse (ops_of lca) (ops_of s1);
+  lastop_diff (ops_of lca) (ops_of s1);
+  inverse_diff_id_s1' (ops_of lca) (ops_of s1) (ops_of s2);
+  assume (forall rid. mem_rid rid (diff (fst (un_snoc (ops_of s1))) (ops_of lca)) ==> ~ (mem_rid rid (diff (ops_of s2) (ops_of lca)))); ()
+
+let exists_triple (last_op:op_t) (l:log)
+  : (b:bool{b = true <==> (exists op. mem op l /\ fst last_op <> fst op /\
+                         (let pre,suf = pre_suf l op in
+                          not (commutative last_op op) /\
+                          Second_then_first? (resolve_conflict last_op op) /\
+                          commutative_seq op suf))}) =
+  existsb (fun (op:op_t) -> mem op l &&  fst last_op <> fst op &&
+                              (let pre,suf = pre_suf l op in
+                              not (commutative last_op op) &&
+                              Second_then_first? (resolve_conflict last_op op) &&
+                              commutative_seq op suf)) l
+                              
+let lem_exists (lastop:op_t) (l:log)
+  : Lemma (requires true)
+          (ensures exists_triple lastop l <==> (Rem? (snd (snd lastop)) /\
+                   (exists op. mem op l /\ Add? (snd (snd op)) /\ get_ele op = get_ele lastop /\ fst op <> fst lastop /\
+                    (let _, suf = pre_suf l op in
+                    (forall r. mem r suf /\ get_ele r = get_ele lastop ==> Add? (snd (snd r)))))))
+  = ()
+
+let fst_t (f,_,_) = f
+let snd_t (_,s,_) = s
+let thr_t (_,_,t) = t
+
+// returns an operation op in l such that
+// 1. last_op and op are non-commutative
+// 2. op is commutative with all the operations in the suffix of l
+// 3. op should be applied after last_op according to resolve_conflict
+#push-options "--z3rlimit 200" 
+let rec find_op (last_op:op_t) (l l1:log)
+  : Pure op_t
+         (requires length l > 0 /\ length l1 > 0 /\
+                   (exists op. mem op l /\ mem op l1 /\ 
+                          fst last_op <> fst op /\ 
+                          not (commutative last_op op) /\
+                          Second_then_first? (resolve_conflict last_op op) /\
+                          (let _, suf = pre_suf l1 op in
+                          commutative_seq op suf)))
+         (ensures (fun op -> mem op l /\ mem op l1 /\ 
+                          fst last_op <> fst op /\
+                          not (commutative last_op op) /\
+                          Second_then_first? (resolve_conflict last_op op) /\
+                          (let _, suf = pre_suf l1 op in
+                          commutative_seq op suf))) (decreases length l) =
+
+ match length l with
+  |1 -> last l
+  |_ -> let pre, op = un_snoc l in
+       if (mem op l1 && fst last_op <> fst op &&
+           not (commutative last_op op) &&
+           Second_then_first? (resolve_conflict last_op op) &&
+           (let _, suf = pre_suf l1 op in
+            commutative_seq op suf)) then op 
+        else (lemma_mem_snoc pre op;
+              find_op last_op pre l1)
+              
+// returns a triple such that 
+// 1. l = (snoc prefix op) ++ suffix
+// 2. last_op and op are non-commutative
+// 3. op is commutative with all the operations in the suffix of l
+// 4. op should be applied after last_op according to resolve_conflict
+let find_triple (last_op:op_t) (l:log{(exists_triple last_op l)}) 
+  : (t:(log & op_t & log) {mem (snd_t t) l /\ (fst_t t, thr_t t) = pre_suf l (snd_t t) /\
+                                is_prefix (fst_t t) l /\ is_suffix (thr_t t) l /\
+                                Seq.equal l ((Seq.snoc (fst_t t) (snd_t t)) ++ (thr_t t)) /\
+                                length l = length (fst_t t) + 1 + length (thr_t t) /\
+
+                                fst last_op <> fst (snd_t t) /\
+                                not (commutative last_op (snd_t t)) /\
+                                Second_then_first? (resolve_conflict last_op (snd_t t)) /\
+                                commutative_seq (snd_t t) (thr_t t)}) =
+  let op = find_op last_op l l in
+  let pre, suf = pre_suf l op in
+  (pre, op, suf)
+
+let lem_eq_is_equiv_st (x:concrete_st) (a b:log)
+  : Lemma (requires (a == b /\ apply_log x a == apply_log x b))
+          (ensures eq (apply_log x a) (apply_log x b))
+          [SMTPat (eq (apply_log x a) (apply_log x b))] = 
+  eq_is_equiv (apply_log x a) (apply_log x b)
+  
+let lem_eq_is_equiv (a b:log)
+  : Lemma (requires (a == b /\ (forall x. apply_log x a == apply_log x b)))
+          (ensures (forall x. eq (apply_log x a) (apply_log x b))) = ()
+
+let rec split_prefix_forall (l:log) (a:log)
+  : Lemma (requires is_prefix l a)
+          (ensures (forall s. (apply_log s a == apply_log (apply_log s l) (diff a l))) /\
+                   (forall e. mem e l ==> mem e a) /\
+                   (Seq.length a > Seq.length l ==> (last a) == (last (diff a l))))
+          (decreases Seq.length l)
+  = match Seq.length l with
+    |0 -> ()
+    |1 -> ()
+    |_ -> split_prefix_forall (tail l) (tail a)
+    
+let lem_eq_is_equiv_c3_st (x:concrete_st) (l:log) (op hd:op_t) (tl:log)
+  : Lemma (requires eq (apply_log x (cons op l)) (apply_log (do x hd) (cons op tl)) /\
+                    eq (apply_log (do x hd) (cons op tl)) (apply_log (do x hd) (snoc tl op)))
+          (ensures eq (apply_log x (cons op l)) (apply_log (do x hd) (snoc tl op)))
+          [SMTPat (eq (apply_log x (cons op l)) (apply_log (do x hd) (snoc tl op)))] = 
+  transitive (apply_log x (cons op l)) 
+             (apply_log (do x hd) (cons op tl))
+             (apply_log (do x hd) (snoc tl op))
+
+let rec lem_equiv_st_foldl_st (a b:concrete_st) (l:log)
+  : Lemma (requires eq a b) 
+          (ensures eq (apply_log a l) (apply_log b l))
+          (decreases length l)
+          [SMTPat (eq (apply_log a l) (apply_log b l))] =
+  match length l with
+  |0 -> ()
+  |_ -> lem_do a b (head l);
+       lem_equiv_st_foldl_st (do a (head l)) (do b (head l)) (tail l)
+       
+let lem_case1 (l:log) (op:op_t)
+  : Lemma (requires commutative_seq op l /\ distinct_ops l /\ length l > 0)
+          (ensures (let hd = head l in let tl = tail l in
+                    (forall x. apply_log x (cons op l) == (apply_log (apply_log x (cons op (create 1 hd))) tl))))
+          (decreases length l) = 
+  let hd = head l in let tl = tail l in
+  assert (is_prefix (cons op (create 1 hd)) (cons op l));
+  assert (cons op l = cons op (cons hd tl));
+  assert (cons op (cons hd tl) = cons op (append (create 1 hd) tl)); 
+  append_assoc (create 1 op) (create 1 hd) tl;
+  assert (cons op (append (create 1 hd) tl) = (cons op (create 1 hd)) ++ tl);
+  assert ((cons op (cons hd tl)) = (cons op (create 1 hd)) ++ tl); 
+  assert (cons op l = (cons op (create 1 hd)) ++ tl);
+
+  lem_is_diff ((cons op (create 1 hd)) ++ tl) (cons op (create 1 hd)) tl;  
+  assert (tl = diff (cons op l) (cons op (create 1 hd)));
+  split_prefix_forall (cons op (create 1 hd)) (cons op l)
+
+let rec lem_seq_foldl_forall (l:log) 
+  : Lemma (requires true)
+          (ensures (forall x. (length l > 0 ==> (apply_log x l == apply_log (do x (head l)) (tail l)) /\
+                                          (apply_log x l == do (apply_log x (fst (un_snoc l))) (last l))) /\
+                         (length l = 0 ==> apply_log x l == x)))
+                   
+                   (decreases length l) =
+  match length l with
+  |0 -> ()
+  |_ -> lem_seq_foldl_forall (tail l)
+  
+let lem_case3 (l:log) (op:op_t)
+  : Lemma (requires commutative_seq op l /\ distinct_ops l /\ length l > 0)
+          (ensures (let hd = head l in let tl = tail l in
+                   (forall x. apply_log x (cons hd (cons op tl)) == (apply_log (do x hd) (cons op tl)))))
+                   (decreases length l) = 
+  let hd = head l in let tl = tail l in
+  assert (head (cons hd (cons op tl)) = hd); 
+  lemma_tl hd (cons op tl);
+  assert (tail (cons hd (cons op tl)) = (cons op tl));
+  lem_seq_foldl_forall (cons hd (cons op tl))
+
+let lem_case4 (l:log) (op:op_t)
+  : Lemma (requires commutative_seq op l /\ distinct_ops l /\ length l > 0)
+          (ensures (let hd = head l in let tl = tail l in
+                   (forall x. apply_log (do x hd) (snoc tl op) == (apply_log x (snoc l op)))))
+          (decreases length l) = 
+  let hd = head l in let tl = tail l in
+  assert (head (cons hd (snoc tl op)) = hd);
+  lemma_tl hd (snoc tl op);
+  lemma_tail_snoc (cons hd tl) op;
+  assert (tail (cons hd (snoc tl op)) = (snoc tl op));
+  lem_seq_foldl_forall (cons hd (snoc tl op))
+
+let lem_equiv_st_foldl (a b:log) (l:log)
+  : Lemma (ensures (forall x. eq (apply_log x a) (apply_log x b) ==>
+                         eq (apply_log (apply_log x a) l) (apply_log (apply_log x b) l))) = ()
+                         
+let lem_case2_help (l:log) (op:op_t) //check
+  : Lemma (requires commutative_seq op l /\ distinct_ops l /\ length l > 0)
+          (ensures (let hd = head l in let tl = tail l in
+                    (forall x. eq (apply_log (apply_log x (cons op (create 1 hd))) tl) 
+                             (apply_log (apply_log x (cons hd (create 1 op))) tl))))
+          (decreases length l) = 
+  let hd = head l in let tl = tail l in
+  commutative_prop op hd;
+  assert (forall x. eq (apply_log x (cons op (create 1 hd))) (apply_log x (cons hd (create 1 op))));
+  lem_equiv_st_foldl (cons op (create 1 hd)) (cons hd (create 1 op)) tl
+
+let lem_case2_help1 (l:log) (op:op_t)
+  : Lemma (requires commutative_seq op l /\ distinct_ops l /\ length l > 0 /\
+                    (let hd = head l in let tl = tail l in
+                    (forall x. eq (apply_log (apply_log x (cons op (create 1 hd))) tl) 
+                             (apply_log (apply_log x (cons hd (create 1 op))) tl))))
+          (ensures (let hd = head l in let tl = tail l in
+                    (forall x. apply_log (apply_log x (cons hd (create 1 op))) tl ==
+                          apply_log x (cons hd (cons op tl))))) = 
+  let hd = head l in let tl = tail l in
+  assert (is_prefix (cons hd (create 1 op)) (cons hd (cons op tl)));
+  append_assoc (create 1 hd) (create 1 op) tl;
+  assert (cons hd (cons op tl) = (cons hd (create 1 op) ++ tl));
+  lem_is_diff (cons hd (cons op tl)) (cons hd (create 1 op)) tl;
+  assert (tl = diff (cons hd (cons op tl)) (cons hd (create 1 op)));
+  split_prefix_forall (cons hd (create 1 op)) (cons hd (cons op tl));
+  ()
+
+let lem_case2 (l:log) (op:op_t)
+  : Lemma (requires commutative_seq op l /\ distinct_ops l /\ length l > 0 /\
+                    (let hd = head l in let tl = tail l in
+                    (forall x. eq (apply_log (apply_log x (cons op (create 1 hd))) tl) 
+                             (apply_log (apply_log x (cons hd (create 1 op))) tl) /\
+                          apply_log (apply_log x (cons hd (create 1 op))) tl ==
+                          apply_log x (cons hd (cons op tl)))))
+          (ensures (let hd = head l in let tl = tail l in
+                    (forall x. eq (apply_log (apply_log x (cons op (create 1 hd))) tl) 
+                             (apply_log x (cons hd (cons op tl)))))) = ()
+
+let rec lem_foldl_comm (l:log) (op:op_t)
+  : Lemma (requires commutative_seq op l /\ distinct_ops l)
+          (ensures (forall x. eq (apply_log x (cons op l)) (apply_log x (snoc l op)))) (decreases length l) =
+  match length l with
+  |0 -> lemma_empty l; 
+       append_empty_r (create 1 op); 
+       append_empty_l (create 1 op);
+       assert (forall x. apply_log x (cons op l) == apply_log x (snoc l op));
+       lem_eq_is_equiv (cons op l) (snoc l op)
+      
+  |_ -> let hd = head l in let tl = tail l in
+       assert (l == cons hd tl);
+       distinct_invert_append (create 1 hd) tl;
+       assert (commutative_seq op tl /\ distinct_ops tl);
+       lem_foldl_comm tl op;  
+       lem_case1 l op; // eq (apply_log x (cons op l)) (seq_foldl (apply_log x (cons op (create 1 hd))) tl))
+       lem_case2_help l op;
+       lem_case2_help1 l op;
+       lem_case2 l op; // eq (apply_log (seq_foldl x (cons op (create 1 hd))) tl) (apply_log x (cons hd (cons op tl))));      
+       lem_case3 l op; // eq (apply_log x (cons hd (cons op tl))) (apply_log (do x hd) (cons op tl)))       
+       assert (forall x. eq (apply_log (do x hd) (cons op tl)) (apply_log (do x hd) (snoc tl op))); // from IH       
+       lem_case4 l op // eq (apply_log (do x hd) (snoc tl op)) (apply_log x (snoc l op)));
+
+let lem_seq_foldl_split (x:concrete_st) (p:log) (s:log)
+  : Lemma (ensures apply_log (apply_log x p) s == (apply_log x (p ++ s)))
+          (decreases length p) =
+  lem_is_diff (p ++ s) p s;
+  split_prefix x p (p ++ s)  
+let lem_seq_foldl_op (x:concrete_st) (l:log) (op:op_t)
+  : Lemma (requires distinct_ops l /\ mem op l /\
+                    (let _, s = pre_suf l op in commutative_seq op s))
+          (ensures (let p,s = pre_suf l op in
+                      eq (apply_log x l) (do (apply_log x (p ++ s)) op)))
+          (decreases length l) = 
+  let pre, suf = pre_suf l op in
+  assert (commutative_seq op suf); 
+  pre_suf_prop l op;
+  lem_foldl_comm suf op;
+  assert (forall x. eq (apply_log x (cons op suf)) (apply_log x (snoc suf op)));
+  split_prefix x pre l;
+  append_assoc pre (create 1 op) suf;
+  assert (l == (snoc pre op) ++ suf /\ l == pre ++ (cons op suf)); 
+  lem_is_diff l pre (cons op suf);
+
+  pre_suf_prop l op;
+  assert (distinct_ops (pre ++ suf));
+  assert (not (mem_id (fst op) (pre ++ suf)));
+  distinct_append pre suf;
+  distinct_append (pre ++ suf) (create 1 op);
+  append_assoc pre suf (create 1 op);
+  assert (distinct_ops (pre ++ (snoc suf op)));
+
+  append_assoc pre suf (create 1 op); 
+  lem_is_diff (snoc (pre ++ suf) op) (pre ++ suf) (create 1 op);
+  assert (is_prefix (pre ++ suf) (snoc (pre ++ suf) op));
+  split_prefix x (pre ++ suf) (snoc (pre ++ suf) op); 
+  assert (length (snoc (pre ++ suf) op) > 0);
+  lem_apply_log x (snoc (pre ++ suf) op);
+  lem_last (snoc (pre ++ suf) op); 
+  un_snoc_snoc (pre ++ suf) op;
+  
+  assert (apply_log x l == apply_log (apply_log x pre) (cons op suf));
+  assert (eq (apply_log x l) (apply_log (apply_log x pre) (snoc suf op))); 
+  lem_seq_foldl_split x pre (snoc suf op);
+
+  assert (apply_log x (snoc (pre ++ suf) op) == do (apply_log x (pre ++ suf)) op);
+  assert (apply_log x (snoc (pre ++ suf) op) == apply_log x (pre ++ (snoc suf op)));
+  assert (apply_log x (pre ++ (snoc suf op)) == apply_log (apply_log x pre) (snoc suf op));
+  
+  assert (apply_log (apply_log x pre) (snoc suf op) == do (apply_log x (pre ++ suf)) op);
+  
+  eq_is_equiv (apply_log (apply_log x pre) (snoc suf op)) (do (apply_log x (pre ++ suf)) op);
+  transitive (apply_log x l) (apply_log (apply_log x pre) (snoc suf op)) (do (apply_log x (pre ++ suf)) op)
+
+// returns the inverse state by undoing operation op in (ops_of s)
+let inverse_st_op (s:st) (op:op_t{mem op (ops_of s) /\ 
+                           (let _, suf = pre_suf (ops_of s) op in
+                            commutative_seq op suf)})
+  : GTot (i:st{(let (pre,suf) = pre_suf (ops_of s) op in
+               eq (v_of s) (do (v_of i) op) /\
+               (ops_of i == (pre ++ suf)) /\
+               (ops_of s == (Seq.snoc pre op) ++ suf) /\
+               is_prefix pre (ops_of s) /\ is_prefix pre (ops_of i) /\
+               length (ops_of i) = length (ops_of s) - 1 /\
+               (forall id. (mem_id id (ops_of i) \/ id = fst op) <==> mem_id id (ops_of s)) /\
+               (forall id. mem_id id (ops_of i) <==> (mem_id id (ops_of s) /\ id <> fst op)))}) = 
+  let pre, suf = pre_suf (ops_of s) op in
+  pre_suf_prop (ops_of s) op;
+  lem_seq_foldl_op init_st (ops_of s) op;
+  let v_i = apply_log init_st (pre ++ suf) in
+  assert (eq (v_of s) (do v_i op));
+  (v_i, hide (pre ++ suf))
+
+#push-options "--z3rlimit 50 --ifuel 3"
+let lem_l2a_l1r_eq''_base (lca s1 s2:st) (last1 last2:op_t)
+  : Lemma (requires ops_of s1 = ops_of lca /\ ops_of s2 = ops_of lca /\
+                    Add? (snd (snd last2)))
+          (ensures eq (do (concrete_merge (v_of lca) (do (v_of s1) last1) (v_of s2)) last2)
+                      (concrete_merge (v_of lca) (do (v_of s1) last1) (do (v_of s2) last2))) = ()
+
+#push-options "--z3rlimit 100"
+let rec lem_l2a_l1r_eq''_s10 (lca s1 s2:st) (last1 last2:op_t)
+  : Lemma (requires ops_of s1 = ops_of lca /\
+                    is_prefix (ops_of lca) (ops_of s2) /\
+                    Add? (snd (snd last2)) /\
+                    get_rid last1 <> get_rid last2)
+          (ensures eq (do (concrete_merge (v_of lca) (do (v_of s1) last1) (v_of s2)) last2)
+                      (concrete_merge (v_of lca) (do (v_of s1) last1) (do (v_of s2) last2)))
+          (decreases %[length (ops_of s2)]) =
+  if ops_of s2 = ops_of lca then
+     lem_l2a_l1r_eq''_base lca s1 s2 last1 last2
+  else 
+    (admit();lem_l2a_l1r_eq''_s10 lca s1 (inverse_st s2) last1 last2) //done below
+
+let rec lem_l2a_l1r_eq'' (lca s1 s2:st) (last1 last2:op_t)
+  : Lemma (requires Add? (snd (snd last2)) /\ Rem? (snd (snd last1)) /\ get_ele last1 = get_ele last2 /\
+                    is_prefix (ops_of lca) (ops_of s1) /\
+                    is_prefix (ops_of lca) (ops_of s2) /\
+                    get_rid last1 <> get_rid last2)
+          (ensures eq (do (concrete_merge (v_of lca) (do (v_of s1) last1) (v_of s2)) last2)
+                      (concrete_merge (v_of lca) (do (v_of s1) last1) (do (v_of s2) last2)))
+          (decreases %[length (ops_of s2); length (ops_of s1)]) = 
+  if ops_of s1 = ops_of lca && ops_of s2 = ops_of lca then
+    lem_l2a_l1r_eq''_base lca s1 s2 last1 last2
+  else if ops_of s1 = ops_of lca then
+    lem_l2a_l1r_eq''_s10 lca s1 s2 last1 last2
+  else (let s1' = inverse_st s1 in
+        lem_inverse (ops_of lca) (ops_of s1); 
+        lem_l2a_l1r_eq'' lca s1' s2 last1 last2; admit())
+
+let linearizable_gt0_s2'_op (lca s1 s2:st)
+  : Lemma (requires consistent_branches_s1s2_gt0 lca s1 s2 /\ 
+                    (let _, last1 = un_snoc (ops_of s1) in
+                    let _, last2 = un_snoc (ops_of s2) in
+                    fst last1 <> fst last2 /\
+                    exists_triple last1 (diff (ops_of s2) (ops_of lca)) /\                   
+                    (let (_, op2, suf2) = find_triple last1 (diff (ops_of s2) (ops_of lca)) in
+                    suf2 == snd (pre_suf (ops_of s2) op2) /\
+                    (let s2' = inverse_st_op s2 op2 in
+                    get_rid last1 <> get_rid op2 /\
+                    consistent_branches lca s1 s2' /\
+                    consistent_branches lca s1 (do_st s2' op2)))))
+     
+          (ensures (let _, last1 = un_snoc (ops_of s1) in
+                    let (pre2, op2, suf2) = find_triple last1 (diff (ops_of s2) (ops_of lca)) in
+                    let s2' = inverse_st_op s2 op2 in                      
+                    eq (do (concrete_merge (v_of lca) (v_of s1) (v_of s2')) op2)
+                       (concrete_merge (v_of lca) (v_of s1) (do (v_of s2') op2)))) = 
+  let _, last1 = un_snoc (ops_of s1) in
+  let pre2, op2, suf2 = find_triple last1 (diff (ops_of s2) (ops_of lca)) in
+  let s2' = inverse_st_op s2 op2 in
+  lem_exists last1 (diff (ops_of s2) (ops_of lca)); 
+  lem_inverse (ops_of lca) (ops_of s1);
+  lem_diff (ops_of s1) (ops_of lca);
+  lem_suf_equal2_last (ops_of lca) (ops_of s1);
+  lem_diff (ops_of s2) (ops_of lca);
+  lem_suf_equal2 (ops_of lca) (ops_of s2) op2;
+  lem_inverse_op (ops_of lca) (ops_of s2) op2;
+  lem_l2a_l1r_eq'' lca (inverse_st s1) s2' last1 op2
+
+////////////////////////////////////////////////////////////////
+
+let rem_add_lastop_neq_ele (lca s1 s2:st)
+  : Lemma (requires Seq.length (ops_of s1) > Seq.length (ops_of lca) /\
+                    consistent_branches_s2_gt0 lca s1 s2 /\
+                    (let _, last2 = un_snoc (ops_of s2) in
+                    let _, last1 = un_snoc (ops_of s1) in
+                    fst last1 <> fst last2 /\
+                    Add? (snd (snd last1)) /\
+                    not (exists_triple last2 (diff (ops_of s1) (ops_of lca))) /\
+                    not (exists_triple last1 (diff (ops_of s2) (ops_of lca)))))
+          (ensures (let _, last2 = un_snoc (ops_of s2) in
+                    let _, last1 = un_snoc (ops_of s1) in
+                    ~ (Rem? (snd (snd last2)) /\ get_ele last1 = get_ele last2))) =
+  let _, last2 = un_snoc (ops_of s2) in
+  let _, last1 = un_snoc (ops_of s1) in
+  let s1' = inverse_st s1 in
+  lemma_mem_snoc (ops_of s1') last1;
+  assert (mem last1 (ops_of s1));
+  lem_last (ops_of s1);
+  assert (last (ops_of s1) = last1);
+  lem_diff (ops_of s1) (ops_of lca);
+  assert (last (diff (ops_of s1) (ops_of lca)) = last1);
+  assert (mem last1 (diff (ops_of s1) (ops_of lca)));
+  let pre, suf = pre_suf (diff (ops_of s1) (ops_of lca)) last1 in
+  lem_lastop_suf_0 (diff (ops_of s1) (ops_of lca)) pre suf last1;
+  assert (length suf = 0);
+  lemma_empty suf; 
+  comm_empty_log last1 suf; 
+  
+  assert (Rem? (snd (snd last2)) /\ get_ele last1 = get_ele last2 ==> commutative_seq last1 suf); 
+  assert (Rem? (snd (snd last2)) /\ get_ele last1 = get_ele last2 ==> not (commutative last1 last2));
+  assert (Rem? (snd (snd last2)) /\ get_ele last1 = get_ele last2 ==> First_then_second? (resolve_conflict last1 last2));
+  assert (Rem? (snd (snd last2)) /\ get_ele last1 = get_ele last2 ==> 
+          (not (commutative last1 last2) /\
+          First_then_second? (resolve_conflict last1 last2) /\
+          commutative_seq last1 suf));
+  assert (Rem? (snd (snd last2)) /\ get_ele last1 = get_ele last2 ==> 
+           exists_triple last2 (diff (ops_of s1) (ops_of lca)));
+  ()
+
+let linearizable_gt0_s1' (lca s1 s2:st)
+  : Lemma (requires consistent_branches_s1s2_gt0 lca s1 s2 /\ 
+                    (let _, last1 = un_snoc (ops_of s1) in
+                     let _, last2 = un_snoc (ops_of s2) in
+                     fst last1 <> fst last2 /\                    
+                     not (exists_triple last1 (diff (ops_of s2) (ops_of lca))) /\
+                     not (exists_triple last2 (diff (ops_of s1) (ops_of lca))) /\
+                     First_then_second? (resolve_conflict last1 last2) /\
+                     consistent_branches lca (inverse_st s1) s2))
+        
+          (ensures (let _, last1 = un_snoc (ops_of s1) in                  
+                    eq (do (concrete_merge (v_of lca) (v_of (inverse_st s1)) (v_of s2)) last1)
+                       (concrete_merge (v_of lca) (v_of s1) (v_of s2)))) =
+  let _, last1 = un_snoc (ops_of s1) in
+  let _, last2 = un_snoc (ops_of s2) in
+  assert (Add? (snd (snd last1)) /\ Rem? (snd (snd last2)) /\ get_ele last1 = get_ele last2);
+  if Rem? (snd (snd last1)) then ()
+    else (assert (Add? (snd (snd last1))); 
+          rem_add_lastop_neq_ele lca s1 s2;
+          assert (~ (Rem? (snd (snd last2)) /\ get_ele last1 = get_ele last2)); ()); 
+  assert (~ (Add? (snd (snd last1)) /\ Rem? (snd (snd last2)) /\ get_ele last1 = get_ele last2)); 
+  ()
+
+////////////////////////////////////////////////////////////////
+
+let lem_l2a''_s20_ind_l1r_eq (lca s1 s2:st) (last2:op_t)
+  : Lemma (requires consistent_branches lca s1 s2 /\
+                    ops_of s2 = ops_of lca /\ 
+                    length (ops_of s1) > length (ops_of lca) /\
+                    (let _, last1 = un_snoc (ops_of s1) in
+                    Add? (snd (snd last2)) /\ Rem? (snd (snd last1)) /\ get_ele last1 = get_ele last2 /\
+                    not (exists_triple last2 (diff (ops_of s1) (ops_of lca)))) /\
+
+                    (let s1' = inverse_st s1 in
+                     consistent_branches lca s1' s2 /\
+                     not (exists_triple last2 (diff (ops_of s1') (ops_of lca))) /\                  
+                     eq (do (concrete_merge (v_of lca) (v_of s1') (v_of s2)) last2)
+                      (concrete_merge (v_of lca) (v_of s1') (do (v_of s2) last2))))
+                     
+          (ensures eq (do (concrete_merge (v_of lca) (v_of s1) (v_of s2)) last2)
+                      (concrete_merge (v_of lca) (v_of s1) (do (v_of s2) last2))) = 
+  let _, last1 = un_snoc (ops_of s1) in
+  assume (get_rid last1 <> get_rid last2); // can be done
+  lem_inverse (ops_of lca) (ops_of s1);
+  lem_diff (ops_of s1) (ops_of lca); 
+  lem_suf_equal2_last (ops_of lca) (ops_of s1); 
+  lem_l2a_l1r_eq'' lca (inverse_st s1) s2 last1 last2
+  
+//#push-options "--z3rlimit 50"
+let lem_l2a''_s20_ind (lca s1 s2:st) (last2:op_t)
+  : Lemma (requires consistent_branches lca s1 s2 /\
+                    ops_of s2 = ops_of lca /\ 
+                    length (ops_of s1) > length (ops_of lca) /\
+                    Add? (snd (snd last2)) /\
+                    not (exists_triple last2 (diff (ops_of s1) (ops_of lca))) /\
+                    
+                    (let s1' = inverse_st s1 in
+                     consistent_branches lca s1' s2 /\
+                     not (exists_triple last2 (diff (ops_of s1') (ops_of lca))) /\                  
+                     eq (do (concrete_merge (v_of lca) (v_of s1') (v_of s2)) last2)
+                      (concrete_merge (v_of lca) (v_of s1') (do (v_of s2) last2))))
+                     
+          (ensures eq (do (concrete_merge (v_of lca) (v_of s1) (v_of s2)) last2)
+                      (concrete_merge (v_of lca) (v_of s1) (do (v_of s2) last2))) = 
+  let _, last1 = un_snoc (ops_of s1) in
+  if Rem? (snd (snd last1)) && get_ele last1 <> get_ele last2 then admit()
+  else if Add? (snd (snd last1)) then admit()
+  else lem_l2a''_s20_ind_l1r_eq lca s1 s2 last2
+#pop-options
+
+let rec lem_l2a''_s20 (lca s1 s2:st) (last2:op_t)
+  : Lemma (requires consistent_branches lca s1 s2 /\
+                    ops_of s2 = ops_of lca /\
+                    Add? (snd (snd last2)) /\
+                    not (exists_triple last2 (diff (ops_of s1) (ops_of lca))))
+          (ensures eq (do (concrete_merge (v_of lca) (v_of s1) (v_of s2)) last2)
+                      (concrete_merge (v_of lca) (v_of s1) (do (v_of s2) last2)))
+          (decreases %[length (ops_of s1)]) = 
+  if ops_of s1 = ops_of lca then ()
+  else 
+    (let s1' = inverse_st s1 in
+     pre1_pre2_s1 lca s1 s2;
+     assert (consistent_branches lca s1' s2);
+     let pre1, last1 = un_snoc (ops_of s1) in
+     let pre1d, last1d = un_snoc (diff (ops_of s1) (ops_of lca)) in
+     lem_diff (ops_of s1) (ops_of lca);
+     assert (last1 = last1d);
+     assert ((diff (ops_of s1') (ops_of lca)) = pre1d);
+       //lem_not_exists_add last2 (diff (ops_of s1) (ops_of lca));
+     assert (not (exists_triple last2 (diff (ops_of s1') (ops_of lca))));
+     lem_inverse (ops_of lca) (ops_of s1);
+     lem_l2a''_s20 lca s1' s2 last2;
+     lem_l2a''_s20_ind lca s1 s2 last2)
+     
+let rec lem_l2a' (lca s1 s2:st) (last2:op_t)
+  : Lemma (requires consistent_branches lca s1 s2 /\
+                    Add? (snd (snd last2)))
+          (ensures eq (do (concrete_merge (v_of lca) (v_of s1) (v_of s2)) last2)
+                      (concrete_merge (v_of lca) (v_of s1) (do (v_of s2) last2))) 
+          (decreases %[length (ops_of s2)]) =
+  if ops_of s2 = ops_of lca then
+    lem_l2a''_s20 lca s1 s2 last2
+  else 
+    (pre1_pre2_s2 lca s1 s2;
+     lem_l2a' lca s1 (inverse_st s2) last2; admit())
+
+let lem_l2a (lca s1 s2:st)
+ : Lemma (requires consistent_branches_s2_gt0 lca s1 s2 /\ 
+                   (let _, last2 = un_snoc (ops_of s2) in
+                    Add? (snd (snd last2)) /\
+                    not (exists_triple last2 (diff (ops_of s1) (ops_of lca))) /\
+                    (let s2' = inverse_st s2 in
+                    is_prefix (ops_of lca) (ops_of s2'))))
+          (ensures (let _, last2 = un_snoc (ops_of s2) in
+                    let s2' = inverse_st s2 in
+                    eq (do (concrete_merge (v_of lca) (v_of s1) (v_of s2')) last2)
+                       (concrete_merge (v_of lca) (v_of s1) (v_of s2)))) =
+   let _, last2 = un_snoc (ops_of s2) in
+   let s2' = inverse_st s2 in
+   pre1_pre2_s2 lca s1 s2;
+   lem_diff (ops_of s2) (ops_of lca); 
+   lem_suf_equal2_last (ops_of lca) (ops_of s2); 
+   lem_l2a' lca s1 s2' last2;
+   //assert (S.mem (fst last2, get_ele last2) (do (concrete_merge (v_of lca) (v_of s1) (v_of s2')) last2));
+   //assert (S.mem (fst last2, get_ele last2) (concrete_merge (v_of lca) (v_of s1) (v_of s2)));
+   ()
+
+let lem_l2r_s10p (lca s1 s2:st)
+  : Lemma (requires consistent_branches_s2_gt0 lca s1 s2 /\ 
+                   (let _, last2 = un_snoc (ops_of s2) in
+                    Rem? (snd (snd last2)) /\
+                    not (exists_triple last2 (diff (ops_of s1) (ops_of lca))) /\
+                   (let s2' = inverse_st s2 in
+                    is_prefix (ops_of lca) (ops_of s2'))))
+          (ensures (let s2' = inverse_st s2 in
+                    let _, last2 = un_snoc (ops_of s2) in
+                    consistent_branches lca s1 s2')) =
+  lastop_diff (ops_of lca) (ops_of s2);
+  inverse_diff_id_s2' (ops_of lca) (ops_of s1) (ops_of s2);
+  lem_id_s2' (ops_of lca) (ops_of s1) (ops_of s2);
+  let s2' = inverse_st s2 in
+  assume (forall rid. mem_rid rid (diff (ops_of s1) (ops_of lca)) ==> ~ (mem_rid rid (diff (ops_of s2') (ops_of lca)))); ()
+
+let lem_common_pre1_s2' (lca s1 s2:st) (last2:op_t)
+  : Lemma (requires consistent_branches_s2_gt0 lca s1 s2 /\
+                    not (mem_id (fst last2) (ops_of s2)) /\
+                    not (mem_id (fst last2) (ops_of lca)) /\
+                    not (mem_id (fst last2) (ops_of s1)) /\
+                   ops_of s1 = ops_of lca /\
+                   not (exists_triple last2 (diff (ops_of s1) (ops_of lca))) /\
+                   is_prefix (ops_of lca) (ops_of s2))
+          (ensures (let s2' = inverse_st s2 in
+                   consistent_branches lca s1 s2' /\ 
+                   not (mem_id (fst last2) (ops_of s2')) /\
+                   is_prefix (ops_of lca) (ops_of s2'))) =
+  lem_inverse (ops_of lca) (ops_of s2);
+  inverse_diff_id_s2' (ops_of lca) (ops_of s1) (ops_of s2);
+  lastop_diff (ops_of lca) (ops_of s2);
+  let s2' = inverse_st s2 in
+  assume (forall rid. mem_rid rid (diff (ops_of s1) (ops_of lca)) ==> ~ (mem_rid rid (diff (ops_of s2') (ops_of lca)))); ()
+
+//#push-options "--z3rlimit 50"
+let rec lem_l2r_s10 (lca s1 s2:st) (last2:op_t)
+ : Lemma (requires consistent_branches lca s1 s2 /\ 
+                   ops_of s1 = ops_of lca /\
+                   Rem? (snd (snd last2)) /\
+                   not (mem_id (fst last2) (ops_of lca)) /\
+                   not (mem_id (fst last2) (ops_of s1)) /\
+                   not (mem_id (fst last2) (ops_of s2)) /\
+                   not (exists_triple last2 (diff (ops_of s1) (ops_of lca))) /\
+                   is_prefix (ops_of lca) (ops_of s2))
+          (ensures eq (do (concrete_merge (v_of lca) (v_of s1) (v_of s2)) last2)
+                      (concrete_merge (v_of lca) (v_of s1) (do (v_of s2) last2)))
+         (decreases %[length (ops_of s2)]) =
+   admit();if ops_of s2 = ops_of lca then ()
+   else 
+     (lem_common_pre1_s2' lca s1 s2 last2;
+      lem_l2r_s10 lca s1 (inverse_st s2) last2; admit())
+#pop-options
+
+let not_add_eq (lca s1 s2:st)
+  : Lemma (requires Seq.length (ops_of s1) > Seq.length (ops_of lca) /\
+                    consistent_branches_s2_gt0 lca s1 s2 /\
+                    (let _, last2 = un_snoc (ops_of s2) in
+                     let _, last1 = un_snoc (ops_of s1) in
+                     Rem? (snd (snd last2)) /\
+                     not (exists_triple last2 (diff (ops_of s1) (ops_of lca))) /\
+                     (let s2' = inverse_st s2 in
+                     is_prefix (ops_of lca) (ops_of s2')))) 
+          (ensures (let _, last2 = un_snoc (ops_of s2) in
+                    let _, last1 = un_snoc (ops_of s1) in
+                    ~ (Add? (snd (snd last1)) /\ get_ele last1 = get_ele last2))) = 
+  let _, last2 = un_snoc (ops_of s2) in
+  let _, last1 = un_snoc (ops_of s1) in
+  lastop_neq (ops_of lca) (ops_of s1) (ops_of s2); 
+  assert (fst last1 <> fst last2);
+
+  let s1' = inverse_st s1 in
+  lemma_mem_snoc (ops_of s1') last1;
+  assert (mem last1 (ops_of s1)); 
+  lem_last (ops_of s1);
+  assert (last (ops_of s1) = last1);
+  lem_diff (ops_of s1) (ops_of lca);
+  assert (last (diff (ops_of s1) (ops_of lca)) = last1);
+  assert (mem last1 (diff (ops_of s1) (ops_of lca)));
+  let pre, suf = pre_suf (diff (ops_of s1) (ops_of lca)) last1 in
+  lem_lastop_suf_0 (diff (ops_of s1) (ops_of lca)) pre suf last1;
+  assert (length suf = 0);
+  lemma_empty suf; 
+  comm_empty_log last1 suf; 
+  assert (commutative_seq last1 suf);
+
+  assert ((Add? (snd (snd last1)) /\ get_ele last1 = get_ele last2) ==> not (commutative last1 last2));
+  //resolve_conflict_prop last2 last1;
+  assert ((Add? (snd (snd last1)) /\ get_ele last1 = get_ele last2) ==> 
+                First_then_second? (resolve_conflict last2 last1));
+  assert ((Add? (snd (snd last1)) /\ get_ele last1 = get_ele last2) ==> 
+                not (commutative last2 last1) /\
+                First_then_second? (resolve_conflict last2 last1) /\
+                commutative_seq last1 suf);
+  assert ((Add? (snd (snd last1)) /\ get_ele last1 = get_ele last2) ==> exists_triple last2 (diff (ops_of s1) (ops_of lca)));
+  assert (~ (Add? (snd (snd last1)) /\ get_ele last1 = get_ele last2)); ()
+
+let lem_l2r_neq_p1 (lca s1 s2:st)
+ : Lemma (requires consistent_branches_s1s2_gt0 lca s1 s2)
+         (ensures consistent_branches_s2_gt0 lca (inverse_st s1) s2) =
+ lem_inverse (ops_of lca) (ops_of s1);
+ inverse_diff_id_s1' (ops_of lca) (ops_of s1) (ops_of s2);
+ lastop_diff (ops_of lca) (ops_of s1);
+ assume (forall rid. mem_rid rid (diff (fst (un_snoc (ops_of s1))) (ops_of lca)) ==> ~ (mem_rid rid (diff (ops_of s2) (ops_of lca)))); ()
+
+let lem_l2r_neq_p2'_help (l:log) (last2:op_t)
+  : Lemma (requires distinct_ops l /\ length l > 0 /\
+                    Rem? (snd (snd last2)) /\
+                   (let l', last1 = un_snoc l in
+                    get_ele last1 <> get_ele last2 /\
+                    exists_triple last2 l'))
+          (ensures exists_triple last2 l) 
+          [SMTPat (let l', last1 = un_snoc l in
+                   (exists_triple last2 l'))] =
+  let l', last1 = un_snoc l in
+  let pre', op', suf' = find_triple last2 l' in
+  lemma_mem_snoc l' last1;
+  assert (mem op' l);
+  let pre, suf = pre_suf l op' in
+  
+  assert ((snoc pre op') ++ suf = snoc ((snoc pre' op') ++ suf') last1);
+  append_assoc (snoc pre' op') suf' (create 1 last1);
+  assert ((snoc pre op') ++ suf = ((snoc pre' op') ++ (snoc suf' last1)));
+  lem_suf_equal4 l op';
+  distinct_invert_append l' (create 1 last1);
+  lem_suf_equal4 l' op';
+
+  not_mem_id l' last1;
+  mem_ele_id op' l;
+  mem_ele_id op' l';
+  lem_id_not_snoc l' suf' last1 op'; 
+  assert (not (mem_id (fst op') (snoc suf' last1)));
+ 
+  count_1 l;
+  assert (count_assoc_fst (fst op') (snoc pre op' ++ suf) = 1);
+  lem_count_1 pre suf pre' (snoc suf' last1) op';
+  
+  assert (length suf = length (snoc suf' last1));
+  lemma_append_inj (snoc pre op') suf (snoc pre' op') (snoc suf' last1);
+  assert (suf = snoc suf' last1);
+  lemma_mem_snoc suf' last1;
+  assert (commutative_seq op' suf); 
+  ()
+  
+let lem_l2r_neq_p2' (l:log) (last2:op_t)
+  : Lemma (requires distinct_ops l /\ length l > 0 /\
+                    Rem? (snd (snd last2)) /\
+                   (let l', last1 = un_snoc l in
+                    get_ele last1 <> get_ele last2))
+          (ensures (let l', last1 = un_snoc l in 
+                    (exists_triple last2 l' ==> exists_triple last2 l) /\
+                    (not (exists_triple last2 l) ==> not (exists_triple last2 l')))) = ()
+                    
+let lem_l2r_neq_p2 (lca s1 s2:st)
+ : Lemma (requires consistent_branches_s2_gt0 lca s1 s2 /\ 
+                   length (ops_of s1) > length (ops_of lca) /\
+                   (let _, last2 = un_snoc (ops_of s2) in
+                    let _, last1 = un_snoc (ops_of s1) in
+                    Rem? (snd (snd last2)) /\ get_ele last1 <> get_ele last2 /\
+                    not (exists_triple last2 (diff (ops_of s1) (ops_of lca))) /\
+                   (let s2' = inverse_st s2 in
+                    is_prefix (ops_of lca) (ops_of s2'))))
+         (ensures (let s1' = inverse_st s1 in
+                   let s2' = inverse_st s2 in
+                   let _, last2 = un_snoc (ops_of s2) in
+                   (lem_l2r_neq_p1 lca s1 s2;
+                    (not (exists_triple last2 (diff (ops_of s1') (ops_of lca))))))) = 
+ lem_l2r_neq_p1 lca s1 s2;
+ let s1' = inverse_st s1 in
+ let _, last2 = un_snoc (ops_of s2) in
+ let pre1, last1 = un_snoc (ops_of s1) in
+ let pre1d, last1d = un_snoc (diff (ops_of s1) (ops_of lca)) in
+ lem_diff (ops_of s1) (ops_of lca);
+ assert (last1 = last1d);
+ assert (get_ele last1d <> get_ele last2);
+ assert ((diff (ops_of s1') (ops_of lca)) = pre1d);
+ lem_l2r_neq_p2' (diff (ops_of s1) (ops_of lca)) last2
+
+//#push-options "--z3rlimit 50"
+let rec lem_l2r (lca s1 s2:st)
+ : Lemma (requires consistent_branches_s2_gt0 lca s1 s2 /\ 
+                   (let _, last2 = un_snoc (ops_of s2) in
+                    Rem? (snd (snd last2)) /\
+                    not (exists_triple last2 (diff (ops_of s1) (ops_of lca))) /\
+                   (let s2' = inverse_st s2 in
+                    is_prefix (ops_of lca) (ops_of s2'))))
+          (ensures (let _, last2 = un_snoc (ops_of s2) in
+                    let s2' = inverse_st s2 in
+                    eq (do (concrete_merge (v_of lca) (v_of s1) (v_of s2')) last2)
+                       (concrete_merge (v_of lca) (v_of s1) (v_of s2))))
+         (decreases %[length (ops_of s1)]) = 
+   let _, last2 = un_snoc (ops_of s2) in
+   if ops_of s1 = ops_of lca then
+     (let s2' = inverse_st s2 in
+      lem_l2r_s10p lca s1 s2;
+      lem_l2r_s10 lca s1 s2' last2) 
+   else 
+     (let _, last1 = un_snoc (ops_of s1) in
+      not_add_eq lca s1 s2;
+      assert (~ (Add? (snd (snd last1)) /\ get_ele last1 = get_ele last2));
+      let s1' = inverse_st s1 in
+      if Rem? (snd (snd last1)) && get_ele last1 = get_ele last2 then
+        (admit();lem_last (ops_of s2);
+         lem_last (ops_of s1))
+         //lem_l2r_l1r_eq lca s1 s2
+      else if get_ele last1 <> get_ele last2 then
+        (admit();lem_inverse (ops_of lca) (ops_of s1);
+         inverse_diff_id_s1' (ops_of lca) (ops_of s1) (ops_of s2);
+         lastop_diff (ops_of lca) (ops_of s1);
+         lem_l2r_neq_p2 lca s1 s2;
+         lem_l2r lca s1' s2;
+         lem_last (ops_of s2);
+         lem_last (ops_of s1))
+      else ())
+//#pop-options
+        
+let linearizable_gt0_s2' (lca s1 s2:st)
+  : Lemma (requires consistent_branches_s1s2_gt0 lca s1 s2 /\ 
+                    (let _, last1 = un_snoc (ops_of s1) in
+                     let _, last2 = un_snoc (ops_of s2) in
+                     fst last1 <> fst last2 /\
+                     not (exists_triple last1 (diff (ops_of s2) (ops_of lca))) /\
+                     not (exists_triple last2 (diff (ops_of s1) (ops_of lca))) /\
+                     Second_then_first? (resolve_conflict last1 last2) /\
+                     consistent_branches lca s1 (inverse_st s2)))
+        
+          (ensures (let _, last2 = un_snoc (ops_of s2) in
+                    eq (do (concrete_merge (v_of lca) (v_of s1) (v_of (inverse_st s2))) last2)
+                       (concrete_merge (v_of lca) (v_of s1) (v_of s2)))) =
+  let _, last2 = un_snoc (ops_of s2) in
+  if Add? (snd (snd last2)) then
+    lem_l2a lca s1 s2
+  else lem_l2r lca s1 s2
+  
+////////////////////////////////////////////////////////////////////////
+(*#push-options "--z3rlimit 50 --ifuel 3"
+let linearizable_s1_0''_base_base (lca s1 s2':st) (last2:op_t)
+  : Lemma (requires //consistent_branches lca s1 (do_st s2' last2) /\
+                    ops_of s1 = ops_of lca /\ ops_of s2' = ops_of lca /\
+                    length (ops_of lca) = 0)
+        
+          (ensures eq (do (v_of s2') last2) (concrete_merge (v_of lca) (v_of s1) (do (v_of s2') last2))) = ()
+
+let linearizable_s1_0''_base_ind (lca s1 s2':st) (last2:op_t)
+  : Lemma (requires //consistent_branches lca s1 (do_st s2' last2) /\
+                    ops_of s1 = ops_of lca /\ ops_of s2' = ops_of lca /\
+                    length (ops_of lca) > 0 /\
+
+                    (let l' = inverse_st lca in
+                    let s1' = inverse_st s1 in
+                    let s2'' = inverse_st s2' in
+                    //consistent_branches l' s1' (do_st s2'' last2) /\
+                    ops_of s1' = ops_of l' /\ ops_of s2'' = ops_of l' /\
+                    eq (do (v_of s2'') last2) (concrete_merge (v_of l') (v_of s1') (do (v_of s2'') last2))))
+
+          (ensures eq (do (v_of s2') last2) (concrete_merge (v_of lca) (v_of s1) (do (v_of s2') last2))) = ()
+
+let merge_pre l a b =
+  (forall e. M.contains (concrete_merge l a b) e ==>
+        (forall id. M.contains (sel (concrete_merge l a b) e) id ==>
+               fst (E.sel (sel a e) id) >= fst (E.sel (sel l e) id) /\
+               fst (E.sel (sel b e) id) >= fst (E.sel (sel l e) id)))
+               
+let linearizable_s1_0''_ind_help (lca s1 s2':st) (last2:op_t)
+  : Lemma (requires //consistent_branches lca s1 (do_st s2' last2) /\
+                    ops_of s1 == ops_of lca /\
+                    length (ops_of s2') > length (ops_of lca) /\
+
+                    (let inv2 = inverse_st s2' in
+                    consistent_branches lca s1 (do_st inv2 last2) /\
+                    eq (do (v_of inv2) last2) (concrete_merge (v_of lca) (v_of s1) (do (v_of inv2) last2))))
+        
+          (ensures (let inv2 = inverse_st s2' in
+                   merge_pre (v_of lca) (v_of s1) (do (v_of inv2) last2) /\
+                   (forall ele. M.contains (v_of lca) ele ==> M.contains (v_of s1) ele /\ M.contains (do (v_of inv2) last2) ele) /\
+                   (forall ele rid. M.contains (v_of lca) ele /\ M.contains (sel (v_of lca) ele) rid ==>
+                               M.contains (sel (v_of s1) ele) rid /\ M.contains (sel (do (v_of inv2) last2) ele) rid))) =
+                     //(forall ele rid. M.contains (concrete_merge (v_of lca) (v_of s1) (do (v_of inv2) last2)) ele /\ M.contains (sel (concrete_merge (v_of lca) (v_of s1) (do (v_of inv2) last2)) ele) rid ==>
+            //                fst (E.sel (sel (v_of s1) ele) rid) >= fst (E.sel (sel (v_of lca) ele) rid) /\
+              //              fst (E.sel (sel (do (v_of inv2) last2) ele) rid) >= fst (E.sel (sel (v_of lca) ele) rid)))) = 
+  let inv2 = inverse_st s2' in
+  split_prefix init_st (ops_of lca) (ops_of (do_st inv2 last2));
+  lem_apply init_st (ops_of lca);
+  lem_apply (v_of lca) (diff (snoc (ops_of inv2) last2) (ops_of lca))
+
+#push-options "--z3rlimit 200"
+let linearizable_s1_0''_ind (lca s1 s2':st) (last2:op_t)
+  : Lemma (requires //consistent_branches lca s1 (do_st s2' last2) /\
+                    ops_of s1 == ops_of lca /\
+                    length (ops_of s2') > length (ops_of lca) /\
+
+                    (let inv2 = inverse_st s2' in
+                    consistent_branches lca s1 (do_st inv2 last2) /\
+                    eq (do (v_of inv2) last2) (concrete_merge (v_of lca) (v_of s1) (do (v_of inv2) last2))))
+        
+          (ensures eq (do (v_of s2') last2) (concrete_merge (v_of lca) (v_of s1) (do (v_of s2') last2))) = 
+  linearizable_s1_0''_ind_help lca s1 s2' last2; 
+  //let inv2 = inverse_st s2' in
+  //assume (merge_pre (v_of lca) (v_of s1) (do (v_of inv2) last2));
+  //assume (merge_pre (v_of lca) (v_of s1) (do (v_of s2') last2));
+  ()
+
+let linearizable_s1_0_s2_0_base (lca s1 s2:st)
+  : Lemma (requires //consistent_branches lca s1 s2 /\
+                    ops_of s1 == ops_of lca /\ ops_of s2 == ops_of lca)       
+          (ensures eq (v_of lca) (concrete_merge (v_of lca) (v_of s1) (v_of s2))) = ()
+
+let linearizable_gt0_base_fts (lca s1 s2:st) (last1 last2:op_t)
+  : Lemma (requires //consistent_branches lca (do_st s1 last1) (do_st s2 last2) /\
+                    //consistent_branches lca s1 s2 /\
+                    ops_of s1 = ops_of lca /\ ops_of s2 = ops_of lca /\
+                    fst last1 <> fst last2 /\
+                    First_then_second? (resolve_conflict last1 last2))
+         
+          (ensures eq (do (concrete_merge (v_of lca) (v_of s1) (do (v_of s2) last2)) last1)
+                      (concrete_merge (v_of lca) (do (v_of s1) last1) (do (v_of s2) last2))) = ()
+
+let linearizable_gt0_base_stf (lca s1 s2:st) (last1 last2:op_t)
+  : Lemma (requires //consistent_branches lca (do_st s1 last1) (do_st s2 last2) /\
+                    //consistent_branches lca s1 s2 /\
+                    ops_of s1 = ops_of lca /\ ops_of s2 = ops_of lca /\
+                    fst last1 <> fst last2 /\
+                    Second_then_first? (resolve_conflict last1 last2))
+         
+          (ensures eq (do (concrete_merge (v_of lca) (do (v_of s1) last1) (v_of s2)) last2)
+                      (concrete_merge (v_of lca) (do (v_of s1) last1) (do (v_of s2) last2))) = ()
+
+let linearizable_gt0_ind_fts (lca s1 s2:st) (last1 last2:op_t)
+  : Lemma (requires //consistent_branches lca (do_st s1 last1) (do_st s2 last2) /\
+                    //consistent_branches lca s1 s2 /\
+                    length (ops_of s2) > length (ops_of lca) /\
+                    fst last1 <> fst last2 /\
+                    (let s2' = inverse_st s2 in
+                    First_then_second? (resolve_conflict last1 last2) /\
+                    //consistent_branches lca s1 (do_st s2' last2) /\
+                    //consistent_branches lca (do_st s1 last1) (do_st s2' last2) /\
+                    //consistent_branches lca s1 (do_st s2 last2) /\
+                    eq (do (concrete_merge (v_of lca) (v_of s1) (do (v_of s2') last2)) last1)
+                       (concrete_merge (v_of lca) (do (v_of s1) last1) (do (v_of s2') last2))))
+       
+          (ensures eq (do (concrete_merge (v_of lca) (v_of s1) (do (v_of s2) last2)) last1)
+                      (concrete_merge (v_of lca) (do (v_of s1) last1) (do (v_of s2) last2))) = ()
+
+let merge_pre_ext l a b =
+  (forall e. M.contains l e ==> M.contains a e /\ M.contains b e) /\
+  (forall e id. M.contains l e /\ M.contains (sel l e) id ==> M.contains (sel a e) id /\ M.contains (sel b e) id) /\
+  (forall e. M.contains (concrete_merge l a b) e ==>
+        (forall id. M.contains (sel (concrete_merge l a b) e) id ==>
+               fst (E.sel (sel a e) id) >= fst (E.sel (sel l e) id) /\
+               fst (E.sel (sel b e) id) >= fst (E.sel (sel l e) id)))
+
+let linearizable_gt0_ind_stf_help (lca s1 s2:st) (last1 last2:op_t)
+  : Lemma (requires //consistent_branches lca (do_st s1 last1) (do_st s2 last2) /\
+                    //consistent_branches lca s1 s2 /\
+                    length (ops_of s2) > length (ops_of lca) /\
+                    fst last1 <> fst last2 /\
+                    (let s2' = inverse_st s2 in
+                    ops_of s1 = ops_of lca /\
+                    Second_then_first? (resolve_conflict last1 last2) /\
+                    //Rem? (snd (snd last1)) /\ Add? (snd (snd last2)) /\
+                    //consistent_branches lca (do_st s1 last1) s2' /\
+                    consistent_branches lca (do_st s1 last1) (do_st s2' last2) /\
+                    //consistent_branches lca (do_st s1 last1) s2 /\
+                    eq (do (concrete_merge (v_of lca) (do (v_of s1) last1) (v_of s2')) last2)
+                       (concrete_merge (v_of lca) (do (v_of s1) last1) (do (v_of s2') last2))))
+        
+          (ensures (let s2' = inverse_st s2 in
+                   merge_pre (v_of lca) (do (v_of s1) last1) (do (v_of s2') last2) /\
+                   (forall ele. M.contains (v_of lca) ele ==> M.contains (do (v_of s1) last1) ele /\ M.contains (do (v_of s2') last2) ele) /\
+                   (forall ele rid. M.contains (v_of lca) ele /\ M.contains (sel (v_of lca) ele) rid ==>
+                               M.contains (sel (do (v_of s1) last1) ele) rid /\ M.contains (sel (do (v_of s2') last2) ele) rid))) =
+  let s2' = inverse_st s2 in
+  split_prefix init_st (ops_of lca) (ops_of (do_st s2' last2));
+  lem_apply init_st (ops_of lca);
+  lem_apply (v_of lca) (diff (snoc (ops_of s2') last2) (ops_of lca));
+  split_prefix init_st (ops_of lca) (ops_of (do_st s1 last1));
+  lem_apply init_st (ops_of lca);
+  lem_apply (v_of lca) (diff (snoc (ops_of s1) last1) (ops_of lca))
+
+let linearizable_gt0_ind_stf_ra (lca s1 s2:st) (last1 last2:op_t)
+  : Lemma (requires //consistent_branches lca (do_st s1 last1) (do_st s2 last2) /\
+                    //consistent_branches lca s1 s2 /\
+                    length (ops_of s2) > length (ops_of lca) /\
+                    fst last1 <> fst last2 /\
+                    get_rid last1 <> get_rid last2 /\
+                    (let s2' = inverse_st s2 in
+                    ops_of s1 = ops_of lca /\
+                    Second_then_first? (resolve_conflict last1 last2) /\
+                    Rem? (snd (snd last1)) /\ Add? (snd (snd last2)) /\ //get_ele last1 <> get_ele last2 /\
+                    //consistent_branches lca (do_st s1 last1) s2' /\
+                    consistent_branches lca (do_st s1 last1) (do_st s2' last2) /\
+                    //consistent_branches lca (do_st s1 last1) s2 /\
+                    eq (do (concrete_merge (v_of lca) (do (v_of s1) last1) (v_of s2')) last2)
+                       (concrete_merge (v_of lca) (do (v_of s1) last1) (do (v_of s2') last2))))
+       
+          (ensures eq (do (concrete_merge (v_of lca) (do (v_of s1) last1) (v_of s2)) last2)
+                      (concrete_merge (v_of lca) (do (v_of s1) last1) (do (v_of s2) last2))) = 
+  let s2' = inverse_st s2 in
+  linearizable_gt0_ind_stf_help lca s1 s2 last1 last2;
+  assert (merge_pre_ext (v_of lca) (do (v_of s1) last1) (do (v_of s2') last2));
+  assert (forall e. M.contains (do (concrete_merge (v_of lca) (do (v_of s1) last1) (v_of s2)) last2) e =
+               M.contains (concrete_merge (v_of lca) (do (v_of s1) last1) (do (v_of s2) last2)) e);
+  assert (forall e rid. M.contains (do (concrete_merge (v_of lca) (do (v_of s1) last1) (v_of s2)) last2) e ==>
+                   M.contains (sel (do (concrete_merge (v_of lca) (do (v_of s1) last1) (v_of s2)) last2) e) rid =
+                   M.contains (sel (concrete_merge (v_of lca) (do (v_of s1) last1) (do (v_of s2) last2)) e) rid); 
+  assert (forall e rid. M.contains (do (concrete_merge (v_of lca) (do (v_of s1) last1) (v_of s2)) last2) e ==>
+                   E.sel (sel (do (concrete_merge (v_of lca) (do (v_of s1) last1) (v_of s2)) last2) e) rid ==
+                   E.sel (sel (concrete_merge (v_of lca) (do (v_of s1) last1) (do (v_of s2) last2)) e) rid);
+  assert (eq (do (concrete_merge (v_of lca) (do (v_of s1) last1) (v_of s2)) last2)
+             (concrete_merge (v_of lca) (do (v_of s1) last1) (do (v_of s2) last2)));
+  ()
+
+let linearizable_gt0_ind_stf_rr (lca s1 s2:st) (last1 last2:op_t)
+  : Lemma (requires //consistent_branches lca (do_st s1 last1) (do_st s2 last2) /\
+                    //consistent_branches lca s1 s2 /\
+                    length (ops_of s2) > length (ops_of lca) /\
+                    fst last1 <> fst last2 /\
+                    get_rid last1 <> get_rid last2 /\
+                    (let s2' = inverse_st s2 in
+                    ops_of s1 = ops_of lca /\
+                    Second_then_first? (resolve_conflict last1 last2) /\
+                    Rem? (snd (snd last1)) /\ Rem? (snd (snd last2)) /\ //get_ele last1 <> get_ele last2 /\
+                    //consistent_branches lca (do_st s1 last1) s2' /\
+                    consistent_branches lca (do_st s1 last1) (do_st s2' last2) /\
+                    //consistent_branches lca (do_st s1 last1) s2 /\
+                    eq (do (concrete_merge (v_of lca) (do (v_of s1) last1) (v_of s2')) last2)
+                       (concrete_merge (v_of lca) (do (v_of s1) last1) (do (v_of s2') last2))))
+       
+          (ensures eq (do (concrete_merge (v_of lca) (do (v_of s1) last1) (v_of s2)) last2)
+                      (concrete_merge (v_of lca) (do (v_of s1) last1) (do (v_of s2) last2))) = 
+  let s2' = inverse_st s2 in
+  linearizable_gt0_ind_stf_help lca s1 s2 last1 last2;
+  assert (merge_pre_ext (v_of lca) (do (v_of s1) last1) (do (v_of s2') last2));
+  assert (forall e. M.contains (do (concrete_merge (v_of lca) (do (v_of s1) last1) (v_of s2)) last2) e =
+               M.contains (concrete_merge (v_of lca) (do (v_of s1) last1) (do (v_of s2) last2)) e); 
+  assert (forall e rid. M.contains (do (concrete_merge (v_of lca) (do (v_of s1) last1) (v_of s2)) last2) e ==>
+                   M.contains (sel (do (concrete_merge (v_of lca) (do (v_of s1) last1) (v_of s2)) last2) e) rid =
+                   M.contains (sel (concrete_merge (v_of lca) (do (v_of s1) last1) (do (v_of s2) last2)) e) rid);
+  assert (forall e rid. M.contains (do (concrete_merge (v_of lca) (do (v_of s1) last1) (v_of s2)) last2) e ==>
+                   E.sel (sel (do (concrete_merge (v_of lca) (do (v_of s1) last1) (v_of s2)) last2) e) rid ==
+                   E.sel (sel (concrete_merge (v_of lca) (do (v_of s1) last1) (do (v_of s2) last2)) e) rid); 
+  assert (eq (do (concrete_merge (v_of lca) (do (v_of s1) last1) (v_of s2)) last2)
+             (concrete_merge (v_of lca) (do (v_of s1) last1) (do (v_of s2) last2)));
+  ()
+
+let linearizable_gt0_ind_stf_ar (lca s1 s2:st) (last1 last2:op_t)
+  : Lemma (requires //consistent_branches lca (do_st s1 last1) (do_st s2 last2) /\
+                    //consistent_branches lca s1 s2 /\
+                    length (ops_of s2) > length (ops_of lca) /\
+                    fst last1 <> fst last2 /\
+                    get_rid last1 <> get_rid last2 /\
+                    (let s2' = inverse_st s2 in
+                    ops_of s1 = ops_of lca /\
+                    Second_then_first? (resolve_conflict last1 last2) /\
+                    Add? (snd (snd last1)) /\ Rem? (snd (snd last2)) /\ get_ele last1 <> get_ele last2 /\
+                    //consistent_branches lca (do_st s1 last1) s2' /\
+                    consistent_branches lca (do_st s1 last1) (do_st s2' last2) /\
+                    //consistent_branches lca (do_st s1 last1) s2 /\
+                    eq (do (concrete_merge (v_of lca) (do (v_of s1) last1) (v_of s2')) last2)
+                       (concrete_merge (v_of lca) (do (v_of s1) last1) (do (v_of s2') last2))))
+       
+          (ensures eq (do (concrete_merge (v_of lca) (do (v_of s1) last1) (v_of s2)) last2)
+                      (concrete_merge (v_of lca) (do (v_of s1) last1) (do (v_of s2) last2))) = 
+  let s2' = inverse_st s2 in
+  linearizable_gt0_ind_stf_help lca s1 s2 last1 last2;
+  assert (merge_pre_ext (v_of lca) (do (v_of s1) last1) (do (v_of s2') last2));
+  assert (forall e. M.contains (do (concrete_merge (v_of lca) (do (v_of s1) last1) (v_of s2)) last2) e =
+               M.contains (concrete_merge (v_of lca) (do (v_of s1) last1) (do (v_of s2) last2)) e);
+  assert (forall e rid. M.contains (do (concrete_merge (v_of lca) (do (v_of s1) last1) (v_of s2)) last2) e ==>
+                   M.contains (sel (do (concrete_merge (v_of lca) (do (v_of s1) last1) (v_of s2)) last2) e) rid =
+                   M.contains (sel (concrete_merge (v_of lca) (do (v_of s1) last1) (do (v_of s2) last2)) e) rid);
+  assert (forall e rid. M.contains (do (concrete_merge (v_of lca) (do (v_of s1) last1) (v_of s2)) last2) e ==>
+                   E.sel (sel (do (concrete_merge (v_of lca) (do (v_of s1) last1) (v_of s2)) last2) e) rid ==
+                   E.sel (sel (concrete_merge (v_of lca) (do (v_of s1) last1) (do (v_of s2) last2)) e) rid);
+  assert (eq (do (concrete_merge (v_of lca) (do (v_of s1) last1) (v_of s2)) last2)
+             (concrete_merge (v_of lca) (do (v_of s1) last1) (do (v_of s2) last2)));
+  ()
+
+let linearizable_gt0_ind_stf_aaa (lca s2:st) (last1 last2:op_t) // s1 = lca
+  : Lemma (requires //consistent_branches lca (do_st s1 last1) (do_st s2 last2) /\
+                    //consistent_branches lca s1 s2 /\
+                    length (ops_of s2) > length (ops_of lca) /\
+                    //fst last1 <> fst last2 /\
+                    get_rid last1 <> get_rid last2 /\
+                    (let s2' = inverse_st s2 in
+                     let _, last2' = un_snoc (ops_of s2) in
+                     Add? (snd (snd last2')) /\
+                    //ops_of s1 = ops_of lca /\
+                    //Second_then_first? (resolve_conflict last1 last2) /\
+                    Add? (snd (snd last1)) /\ Add? (snd (snd last2)) /\ //get_ele last1 = get_ele last2 /\
+                    //consistent_branches lca (do_st s1 last1) s2' /\
+                    consistent_branches lca (do_st lca last1) (do_st s2' last2) /\
+                    //consistent_branches lca (do_st s1 last1) s2 /\
+                    eq (do (concrete_merge (v_of lca) (do (v_of lca) last1) (v_of s2')) last2)
+                       (concrete_merge (v_of lca) (do (v_of lca) last1) (do (v_of s2') last2))))
+       
+          (ensures eq (do (concrete_merge (v_of lca) (do (v_of lca) last1) (v_of s2)) last2)
+                      (concrete_merge (v_of lca) (do (v_of lca) last1) (do (v_of s2) last2))) = 
+  let s2' = inverse_st s2 in
+  linearizable_gt0_ind_stf_help lca lca s2 last1 last2;
+  assert (merge_pre_ext (v_of lca) (do (v_of lca) last1) (do (v_of s2') last2));
+  assert (forall e. M.contains (do (concrete_merge (v_of lca) (do (v_of lca) last1) (v_of s2)) last2) e =
+               M.contains (concrete_merge (v_of lca) (do (v_of lca) last1) (do (v_of s2) last2)) e);
+  assert (forall e rid. M.contains (do (concrete_merge (v_of lca) (do (v_of lca) last1) (v_of s2)) last2) e ==>
+                   M.contains (sel (do (concrete_merge (v_of lca) (do (v_of lca) last1) (v_of s2)) last2) e) rid =
+                   M.contains (sel (concrete_merge (v_of lca) (do (v_of lca) last1) (do (v_of s2) last2)) e) rid);
+  assert (forall e rid. (e = get_ele last2 /\  M.contains (do (concrete_merge (v_of lca) (do (v_of lca) last1) (v_of s2)) last2) e) ==>
+                   E.sel (sel (do (concrete_merge (v_of lca) (do (v_of lca) last1) (v_of s2)) last2) e) rid ==
+                   E.sel (sel (concrete_merge (v_of lca) (do (v_of lca) last1) (do (v_of s2) last2)) e) rid);
+  assert (eq (do (concrete_merge (v_of lca) (do (v_of lca) last1) (v_of s2)) last2)
+             (concrete_merge (v_of lca) (do (v_of lca) last1) (do (v_of s2) last2)));
+  ()
+
+let linearizable_gt0_ind_stf_aar (lca s2:st) (last1 last2:op_t) // s1 = lca
+  : Lemma (requires //consistent_branches lca (do_st s1 last1) (do_st s2 last2) /\
+                    //consistent_branches lca s1 s2 /\
+                    length (ops_of s2) > length (ops_of lca) /\
+                    //fst last1 <> fst last2 /\
+                    get_rid last1 <> get_rid last2 /\
+                    (let s2' = inverse_st s2 in
+                     let _, last2' = un_snoc (ops_of s2) in
+                     Rem? (snd (snd last2')) /\
+                    //ops_of s1 = ops_of lca /\
+                    //Second_then_first? (resolve_conflict last1 last2) /\
+                    Add? (snd (snd last1)) /\ Add? (snd (snd last2)) /\ //get_ele last1 = get_ele last2 /\
+                    //consistent_branches lca (do_st s1 last1) s2' /\
+                    consistent_branches lca (do_st lca last1) (do_st s2' last2) /\
+                    //consistent_branches lca (do_st s1 last1) s2 /\
+                    eq (do (concrete_merge (v_of lca) (do (v_of lca) last1) (v_of s2')) last2)
+                       (concrete_merge (v_of lca) (do (v_of lca) last1) (do (v_of s2') last2))))
+       
+          (ensures eq (do (concrete_merge (v_of lca) (do (v_of lca) last1) (v_of s2)) last2)
+                      (concrete_merge (v_of lca) (do (v_of lca) last1) (do (v_of s2) last2))) = 
+  let s2' = inverse_st s2 in
+  linearizable_gt0_ind_stf_help lca lca s2 last1 last2;
+  assert (merge_pre_ext (v_of lca) (do (v_of lca) last1) (do (v_of s2') last2));
+  assert (forall e. M.contains (do (concrete_merge (v_of lca) (do (v_of lca) last1) (v_of s2)) last2) e =
+               M.contains (concrete_merge (v_of lca) (do (v_of lca) last1) (do (v_of s2) last2)) e);
+  assert (forall e rid. M.contains (do (concrete_merge (v_of lca) (do (v_of lca) last1) (v_of s2)) last2) e ==>
+                   M.contains (sel (do (concrete_merge (v_of lca) (do (v_of lca) last1) (v_of s2)) last2) e) rid =
+                   M.contains (sel (concrete_merge (v_of lca) (do (v_of lca) last1) (do (v_of s2) last2)) e) rid);
+  assert (forall e rid. (e = get_ele last2 /\  M.contains (do (concrete_merge (v_of lca) (do (v_of lca) last1) (v_of s2)) last2) e) ==>
+                   E.sel (sel (do (concrete_merge (v_of lca) (do (v_of lca) last1) (v_of s2)) last2) e) rid ==
+                   E.sel (sel (concrete_merge (v_of lca) (do (v_of lca) last1) (do (v_of s2) last2)) e) rid);
+  assert (eq (do (concrete_merge (v_of lca) (do (v_of lca) last1) (v_of s2)) last2)
+             (concrete_merge (v_of lca) (do (v_of lca) last1) (do (v_of s2) last2)));
+  ()
+  
+let linearizable_gt0_ind1_fts (lca s1 s2:st) (last1 last2:op_t)
+  : Lemma (requires //consistent_branches lca (do_st s1 last1) (do_st s2 last2) /\
+                    //consistent_branches lca s1 s2 /\
+                    length (ops_of s1) > length (ops_of lca) /\
+                    fst last1 <> fst last2 /\
+                    (let s1' = inverse_st s1 in
+                    ops_of s2 = ops_of lca /\
+                    First_then_second? (resolve_conflict last1 last2) /\
+                    //consistent_branches lca s1' (do_st s2 last2) /\
+                    //consistent_branches lca (do_st s1' last1) (do_st s2 last2) /\
+                    //consistent_branches lca s1 (do_st s2 last2) /\
+                    eq (do (concrete_merge (v_of lca) (v_of s1') (do (v_of s2) last2)) last1)
+                       (concrete_merge (v_of lca) (do (v_of s1') last1) (do (v_of s2) last2))))
+                           
+          (ensures eq (do (concrete_merge (v_of lca) (v_of s1) (do (v_of s2) last2)) last1)
+                      (concrete_merge (v_of lca) (do (v_of s1) last1) (do (v_of s2) last2))) = ()
+
+let linearizable_gt0_ind1_stf_help (lca s1 s2:st) (last1 last2:op_t)
+  : Lemma (requires length (ops_of s1) > length (ops_of lca) /\
+                    (let s1' = inverse_st s1 in
+                    consistent_branches lca (do_st s1' last1) (do_st s2 last2) /\
+                    eq (do (concrete_merge (v_of lca) (do (v_of s1') last1) (v_of s2)) last2)
+                       (concrete_merge (v_of lca) (do (v_of s1') last1) (do (v_of s2) last2))))
+        
+          (ensures (let s1' = inverse_st s1 in
+                   merge_pre (v_of lca) (do (v_of s1') last1) (do (v_of s2) last2) /\
+                   (forall ele. M.contains (v_of lca) ele ==> M.contains (do (v_of s1') last1) ele /\ M.contains (do (v_of s2) last2) ele) /\
+                   (forall ele rid. M.contains (v_of lca) ele /\ M.contains (sel (v_of lca) ele) rid ==>
+                               M.contains (sel (do (v_of s1') last1) ele) rid /\ M.contains (sel (do (v_of s2) last2) ele) rid))) =
+  let s1' = inverse_st s1 in
+  split_prefix init_st (ops_of lca) (ops_of (do_st s1' last1));
+  lem_apply init_st (ops_of lca);
+  lem_apply (v_of lca) (diff (snoc (ops_of s1') last1) (ops_of lca));
+  split_prefix init_st (ops_of lca) (ops_of (do_st s2 last2));
+  lem_apply init_st (ops_of lca);
+  lem_apply (v_of lca) (diff (snoc (ops_of s2) last2) (ops_of lca))
+  
+let linearizable_gt0_ind1_stf_rr (lca s1 s2:st) (last1 last2:op_t)
+  : Lemma (requires //consistent_branches lca (do_st s1 last1) (do_st s2 last2) /\
+                    //consistent_branches lca s1 s2 /\
+                    length (ops_of s1) > length (ops_of lca) /\
+                    //fst last1 <> fst last2 /\
+                    get_rid last1 <> get_rid last2 /\
+                    Rem? (snd (snd last1)) /\ Rem? (snd (snd last2)) /\
+                    (let s1' = inverse_st s1 in
+                     let _, last1' = un_snoc (ops_of s1) in
+                     Add? (snd (snd last1')) /\
+                    //Second_then_first? (resolve_conflict last1 last2) /\
+                    //consistent_branches lca (do_st s1' last1) s2 /\
+                    //consistent_branches lca (do_st s1' last1) (do_st s2 last2) /\
+                    //consistent_branches lca (do_st s1 last1) s2 /\
+                    eq (do (concrete_merge (v_of lca) (do (v_of s1') last1) (v_of s2)) last2)
+                       (concrete_merge (v_of lca) (do (v_of s1') last1) (do (v_of s2) last2))))
+                           
+          (ensures eq (do (concrete_merge (v_of lca) (do (v_of s1) last1) (v_of s2)) last2)
+                      (concrete_merge (v_of lca) (do (v_of s1) last1) (do (v_of s2) last2))) = 
+  let s1' = inverse_st s1 in
+  //linearizable_gt0_ind1_stf_help lca s1 s2 last1 last2;
+  assume (merge_pre_ext (v_of lca) (do (v_of s1') last1) (do (v_of s2) last2));
+  assume (forall e. M.contains (do (concrete_merge (v_of lca) (do (v_of s1) last1) (v_of s2)) last2) e =
+               M.contains (concrete_merge (v_of lca) (do (v_of s1) last1) (do (v_of s2) last2)) e);
+  assume (forall e rid. M.contains (do (concrete_merge (v_of lca) (do (v_of s1) last1) (v_of s2)) last2) e ==>
+                   M.contains (sel (do (concrete_merge (v_of lca) (do (v_of s1) last1) (v_of s2)) last2) e) rid =
+                   M.contains (sel (concrete_merge (v_of lca) (do (v_of s1) last1) (do (v_of s2) last2)) e) rid);
+  assert (forall e rid. M.contains (do (concrete_merge (v_of lca) (do (v_of s1) last1) (v_of s2)) last2) e ==>
+                   E.sel (sel (do (concrete_merge (v_of lca) (do (v_of s1) last1) (v_of s2)) last2) e) rid ==
+                   E.sel (sel (concrete_merge (v_of lca) (do (v_of s1) last1) (do (v_of s2) last2)) e) rid);  admit();
+  assert (eq (do (concrete_merge (v_of lca) (do (v_of s1) last1) (v_of s2)) last2)
+             (concrete_merge (v_of lca) (do (v_of s1) last1) (do (v_of s2) last2)));
+  ()
+
+
+let linearizable_gt0_ind1_stf_de (lca s1 s2:st) (last1 last2:op_t)
+  : Lemma (requires //consistent_branches lca (do_st s1 last1) (do_st s2 last2) /\
+                    //consistent_branches lca s1 s2 /\
+                    length (ops_of s1) > length (ops_of lca) /\
+                    fst last1 <> fst last2 /\
+                    Disable? (snd (snd last1)) /\ Enable? (snd (snd last2)) /\
+                    (let s1' = inverse_st s1 in
+                    Second_then_first? (resolve_conflict last1 last2) /\
+                    //consistent_branches lca (do_st s1' last1) s2 /\
+                    //consistent_branches lca (do_st s1' last1) (do_st s2 last2) /\
+                    //consistent_branches lca (do_st s1 last1) s2 /\
+                    eq (do (concrete_merge (v_of lca) (do (v_of s1') last1) (v_of s2)) last2)
+                       (concrete_merge (v_of lca) (do (v_of s1') last1) (do (v_of s2) last2))))
+                           
+          (ensures eq (do (concrete_merge (v_of lca) (do (v_of s1) last1) (v_of s2)) last2)
+                      (concrete_merge (v_of lca) (do (v_of s1) last1) (do (v_of s2) last2))) = ()
 
 ////////////////////////////////////////////////////////////////
 //// Linearization properties - intermediate merge //////
@@ -77,7 +1444,7 @@ let prop1 (l:concrete_st) (o1 o2 o3:op_t)
   : Lemma (requires fst o1 <> fst o3 /\ fst o2 <> fst o3 /\ 
                     resolve_conflict o1 o3 = First_then_second /\
                     resolve_conflict o2 o3 = First_then_second)
-                    //get_rid o1 = get_rid o2 /\ get_rid o3 <> get_rid o1*))
+                    //get_rid o1 = get_rid o2 /\ get_rid o3 <> get_rid o1))
           (ensures eq (concrete_merge (do l o1) (do (do l o1) o2) (do (do l o3) o1)) (do (do (do l o3) o1) o2)) = ()
 
 #push-options "--z3rlimit 50"
